---
layout: simple
title: ［基础知识］连续介质力学数学基础
date: 2017-03-31
category: comsol
---

<script type="text/x-mathjax-config">MathJax.Hub.Config({tex2jax: {inlineMath:[['$','$']]}});</script>
<script type="text/javascript" src="http://cdn.mathjax.org/mathjax/latest/MathJax.js?config=TeX-AMS-MML_HTMLorMML"></script>



\begin{enumerate}
\item Extensional transformation matrix

$
A =
\begin{pmatrix}             
  2 & 0 \\
  0 & 4 \\
\end{pmatrix}
$

Then check the solution for each corner of the original region:

$$\begin{bmatrix}             
  2 & 0 \\
  0 & 4 \\
\end{bmatrix}$$

$\begin{bmatrix}
0\\
0\\
\end{bmatrix}
=
\begin{pmatrix}
0 & 0
\end{pmatrix}
^{\mathrm T}$

,
$\begin{bmatrix}             
  2 & 0 \\
  0 & 4 \\
\end{bmatrix}
\begin{bmatrix}
1\\0
\end{bmatrix}
=
\begin{pmatrix}
2 & 0
\end{pmatrix}
^{\mathrm T}$
,

$\begin{bmatrix}             
  2 & 0 \\
  0 & 4 \\
\end{bmatrix}
\begin{bmatrix}
0\\1
\end{bmatrix}
=
\begin{pmatrix}
0 & 4
\end{pmatrix}
^{\mathrm T}$
,
$\begin{bmatrix}             
  2 & 0 \\
  0 & 4 \\
\end{bmatrix}
\begin{bmatrix}
1\\1
\end{bmatrix}
=
\begin{pmatrix}
2 & 4
\end{pmatrix}
^{\mathrm T}$.

\item Shear transformation matrix 
$\mathbf B =
\begin{pmatrix}             
  3 & 2 \\
  2 & 3 \\
\end{pmatrix}$

Then check the solution for each corner of the original region:

$\begin{bmatrix}             
  3 & 2 \\
  2 & 3 \\
\end{bmatrix}
\begin{bmatrix}
0\\0
\end{bmatrix}
=
\begin{pmatrix}
0 & 0
\end{pmatrix}
^{\mathrm T}$
,
$\begin{bmatrix}             
  3 & 2 \\
  2 & 3 \\
\end{bmatrix}
\begin{bmatrix}
1\\0
\end{bmatrix}
=
\begin{pmatrix}
3 & 2
\end{pmatrix}
^{\mathrm T}$
,

$\begin{bmatrix}             
  3 & 2 \\
  2 & 3 \\
\end{bmatrix}
\begin{bmatrix}
0\\1
\end{bmatrix}
=
\begin{pmatrix}
2 & 3
\end{pmatrix}
^{\mathrm T}$
,
$\begin{bmatrix}             
  3 & 2 \\
  2 & 3 \\
\end{bmatrix}
\begin{bmatrix}
1\\1
\end{bmatrix}
=
\begin{pmatrix}
5 & 5
\end{pmatrix}
^{\mathrm T}$.


\item $\mathbf v' = \mathbf{A B v} = 
\begin{bmatrix}             
  2 & 0 \\
  0 & 4 \\
\end{bmatrix}
\begin{bmatrix}             
  3 & 2 \\
  2 & 3 \\
\end{bmatrix}
\mathbf v
=
\begin{bmatrix}             
  6 & 4 \\
  8 & 12 \\
\end{bmatrix}
\mathbf v
=
\begin{bmatrix}             
  1\\2
\end{bmatrix}
$
\end{enumerate}

\begin{equation}
	\begin{cases}
		6x + 4y = 1,\\[1mm]
		8x + 12y = 2\\
	\end{cases}
	\therefore
	\begin{cases}
		x = 0.1,\\[1mm]
		y = 0.1\\
	\end{cases}
\therefore 
\mathbf v
=
\begin{pmatrix}             
  0.1 & 0.1
\end{pmatrix}
^{\mathrm T}
\end{equation}

\subsection{}
\begin{equation}
det(\lambda \mathbf I - \mathbf A) = det
\begin{bmatrix}             
  \lambda-1 & 1 & 0\\
  1 & \lambda-2 & 1\\
  0 & 1 & \lambda-1
\end{bmatrix}
=\lambda (\lambda-1) (\lambda-3)
=0
\ \ 
\therefore
\begin{cases}
\lambda_1=0, \\ \lambda_2=1, \\ \lambda_3 = 3
\end{cases}
\end{equation}

for $\lambda_1 = 0, 
\begin{bmatrix}             
  -1 & 1 & 0\\
  1 & -2 & 1\\
  0 & 1 & -1
\end{bmatrix}
\mathbf x = 0
\therefore \mathbf x_1 = 
\begin{pmatrix}             
  1 & 1 & 1
\end{pmatrix}
^{\mathrm T}$

for $\lambda_2 = 1, 
\begin{bmatrix}             
  0 & 1 & 0\\
  1 & -1 & 1\\
  0 & 1 & -0
\end{bmatrix}
\mathbf x = 0
\therefore \mathbf x_2 = 
\begin{pmatrix}             
  1 & 0 & -1
\end{pmatrix}
^{\mathrm T}$

for $\lambda_3 = 3, 
\begin{bmatrix}             
  2 & 1 & 0\\
  1 & 1 & 1\\
  0 & 1 & 2
\end{bmatrix}
\mathbf x = 0
\therefore \mathbf x_3 = 
\begin{pmatrix}             
  1 & -2 & 1
\end{pmatrix}
^{\mathrm T}$
\\

Eigenvalues: $\lambda_1=0, \ \lambda_2=1, \ \lambda_3 = 3$

Eigenvectors: 
$\mathbf x_1 =
\begin{pmatrix}             
  1 & 1 & 1
\end{pmatrix}
^{\mathrm T}, \
\mathbf x_2 = 
\begin{pmatrix}             
  1 & 0 & -1
\end{pmatrix}
^{\mathrm T}, \ 
\mathbf x_3 =
\begin{pmatrix}             
  1 & -2 & 1
\end{pmatrix}
^{\mathrm T}
$

\section{Fourier Series}
\subsection{}
f(x) is an even function, $T = 2, \ \omega = \frac{2\pi}{2} = \pi$.

$$f(x)= \frac12 a_0 + \sum_{n=1}^{\infty} a_n \cos (n\pi x)$$

$$a_0 = \frac42 \int_0^1 f(x) dx = 2\int_0^1(1-x^2)dx = 2\left[ x-\frac{x^3}{3} \right]_0^1 = \frac43$$

\begin{equation}
\begin{aligned}
a_n & = 2 \int_0^1 (1-x^2)\cos (n\pi x) dx \\
& =  2\left[ (\frac{1-x^2}{n\pi} + \frac{2}{n^3\pi^3}) \sin (n \pi x) - \frac{2x}{n^2\pi^2}\cos (n \pi x) \right]_0^1\\
& = 2 (-\frac{2}{n^2 \pi^2} \cos\ n\pi) = \frac{4}{n^2 \pi^2} (-1)^{n+1}
\end{aligned}
\end{equation}

\begin{equation}
\begin{aligned}
\therefore
f(x) & = \frac23 + \sum_{n=1}^{\infty} (-1)^{n+1} \frac{4}{n^2 \pi^2} \cos (n \pi x) \\
& \approx \frac 23 + \frac{4}{\pi^2} \cos (\pi x) - \frac{4}{4 \pi^2} \cos (2\pi x)
\end{aligned}
\end{equation}

\subsection{}
f(x) is an even function, $T = 2\pi, \ \omega = \frac{2\pi}{2\pi} = 1$.

$$f(x)= \frac12 a_0 + \sum_{n=1}^{\infty} a_n \cos (n x)$$

$$a_0 = \frac{4}{2\pi} \int_0^{\pi} f(x) dx = \frac{2}{\pi}\int_0^{\pi}\sin(\frac x2)dx = \frac 2 \pi \left[ -2\cos(\frac x 2) \right]_0^\pi = \frac4 \pi$$

\begin{equation}
\begin{aligned}
a_n & = \frac{2}{\pi}\int_0^{\pi}\sin(\frac x2)\cos (nx)dx \\
& =  \frac 2 \pi \left[ \frac{\cos(nx-x/2)}{2n-1} - \frac{\cos(nx+x/2)}{2n+1} \right]_0^\pi\\
& = \frac 2 \pi \left[ \frac{\sin(n\pi)}{2n-1} + \frac{\sin(n\pi)}{2n+1} -(\frac{1}{2n-1} - \frac{1}{2n+1})\right] \\
& = \frac{4}{\pi(1-4n^2)}
\end{aligned}
\end{equation}

\begin{equation}
\begin{aligned}
\therefore
f(x) & = \frac2\pi + \sum_{n=1}^{\infty} \frac{4}{\pi(1-4n^2)} \cos (n \pi x) \\
& \approx \frac 2\pi - \frac{4}{3\pi} \cos (\pi x) - \frac{4}{15\pi} \cos (2\pi x)
\end{aligned}
\end{equation}
\section{Solution Techniques for ODEs}
\begin{enumerate}
\item
from $y'' + 3y' + 2y = 0$, we get 
$\lambda^2 + 3\lambda + 2 = 0$

$\therefore \lambda_1= -1, \lambda_2= -2 \ \ $
$\therefore y=Ae^{-x}+Be^{-2x}$
\item
from $y'' -6y' + 9y = 0$, we get 
$\lambda^2 -6 \lambda + 9 = 0$

$\therefore \lambda_1= \lambda_2= 3 \ \ $
$\therefore y=Ae^{3x}$

\item
from $y'' + 6y' + 9y = 0$, we get 
$\lambda^2 + 6\lambda + 9 = 0$

$\therefore \lambda_1= \lambda_2= -3 \ \ $
$\therefore y=Ae^{-3x}$
\end{enumerate}
\section{Solution Techniques for PDEs}
\subsection{}
Now $AC - B^2 = 0$ in this case, so the equation is parabolic.

Solutions of parabolic equation smooth out as the transformed time variable increases.

The parabolic equation will have unique, stable solution if the Dirichlet or Neumann conditions are applied respectively.
It will be overspecified if the boundary is closed or the Cauchy conditions are applied.

\subsection{}
We express T(x, t) as :
T(x, t) = F(x)G(t)

$$\therefore F(x)\frac{dG(t)}{dt} = \alpha^2 G(t) \frac{d^2 F(x)}{dx^2}$$

By rearrangement we have :
$$\frac{1}{\alpha^2 G(t)} \frac{dG(t)}{dt} = \frac{1}{F(x)} \frac{d^2 F(x)}{dx^2}$$

Since each side of the equation is a function of a dierent variable,they both equal a constant.
$$\frac{1}{\alpha^2 G(t)} \frac{dG(t)}{dt} = \frac{1}{F(x)} \frac{d^2 F(x)}{dx^2} = k$$

\begin{equation}
\therefore
\begin{cases}
\frac{d^2 F(x)}{dx^2} - kF(x) = 0 \\[1mm]
\frac{dG(t)}{dt} - \alpha^2 G(x) = 0
\end{cases}
\end{equation}

\begin{enumerate}
\item
for $k=0$, $F (x) = Ax + B, G(t) = C$
with A, B, C all constants.

Applying boundary and initial conditions gives u(x,t) = 0 which is not what we are looking for.

\item
for $k=+p^2$, $F (x) = A e^{px} + B e^{-px}$

Applying boundary and initial conditions gives F(x) = 0 which leads to u(x, t) = 0.

\item
for $k=-p^2$, $F(x)=A\sin(px)+B\cos(px)$

$\because T (t, 0) = 0$ $\therefore F(0) = B = 0$

$\because T (t, 1) = 0$ $\therefore F(1) = A\sin p + B\cos p = A\sin p = 0$

since $A \ne 0, \ \sin p = 0$ , hence $p = n\pi$ where n = 1,2,...

$\therefore F(x) = A_n \sin(n\pi x)$

$\because \frac{dG(t)}{dt} = p^2 \alpha^2 G(x)
\therefore G_n(t) = C e^{- p^2 \alpha^2 t} = C_n e^{- n^2 \pi^2 \alpha^2 t}$


\end{enumerate}

$$T(x,t) = \sum_{n=1}^{\infty} F_n(x) G_n(t) = \sum_{n=1}^{\infty} C_n \sin(n\pi x) e^{- n^2 \pi^2 \alpha^2 t}$$

$\because T(0,x) = f(x)\  \ \therefore \sum_{n=1}^{\infty} C_n \sin(n\pi x) = f(x)$

Now if we multiply both sides this equation by $\sin (m\pi x)$ and integrate:

$\sum_{n=1}^{\infty} C_n \int_0^1 \sin(n\pi x) \sin (m\pi x)= \int_0^1 f(x) \sin (m\pi x)$

$\because \int_0^1 \sin(n\pi x) \sin(m\pi x) dx = \frac{\delta}{2}$
$\therefore C_n \cdot \frac{1}{2} = \int_0^1 f(x) \sin(n\pi x) dx$

we get the final solution:
\begin{equation}
\begin{cases}
T(x,t) =\sum_{n=1}^{\infty} C_n \sin(n\pi x) e^{- n^2 \pi^2 \alpha^2 t}\\[1mm]
C_n = 2\int_0^1 f(x) \sin(n\pi x) dx
\end{cases}
\end{equation}

\subsection{}
We express T(x, t) as :
T(x, t) = F(x)G(t)

$$\therefore F(x)\frac{dG(t)}{dt} = \alpha^2 G(t) \frac{d^2 F(x)}{dx^2}$$

By rearrangement we have :
$$\frac{1}{\alpha^2 G(t)} \frac{dG(t)}{dt} = \frac{1}{F(x)} \frac{d^2 F(x)}{dx^2}$$

Since each side of the equation is a function of a dierent variable,they both equal a constant.
$$\frac{1}{\alpha^2 G(t)} \frac{dG(t)}{dt} = \frac{1}{F(x)} \frac{d^2 F(x)}{dx^2} = k$$

\begin{equation}
\therefore
\begin{cases}
\frac{d^2 F(x)}{dx^2} - kF(x) = 0 \\[1mm]
\frac{dG(t)}{dt} - \alpha^2 G(x) = 0
\end{cases}
\end{equation}

\begin{enumerate}
\item
for $k=0$, $F (x) = Ax + B, G(t) = C$
with A, B, C all constants.

Applying boundary and initial conditions gives u(x,t) = 0 which is not what we are looking for.


\item
for $k=+p^2$, $F (x) = A e^{px} + B e^{-px}$

Applying boundary and initial conditions gives A=B=0, F(x) = 0 which leads to u(x, t) = 0.

\item
for $k=-p^2$, $F(x)=A\sin(px)+B\cos(px)$

$F_x = Ap \cos(px)- Bp \sin(px)$

$\because T_x (t, 0) = 0$ $\therefore F_x(0) = Ap = 0$, since $p \ne 0, \ A = 0$

$\because T_x (t, 1) = 0$ $\therefore F_x(1) = Ap \cos p- Bp \sin p = - Bp \sin p = 0$

since $B \ne 0, \ \sin p = 0$ , hence $p = n\pi$ where n = 1,2,...

$\therefore F(x) = B_n \cos(n\pi x)$

$\because \frac{dG(t)}{dt} = p^2 \alpha^2 G(x)
\therefore G_n(t) = C e^{- p^2 \alpha^2 t} = C_n e^{- n^2 \pi^2 \alpha^2 t}$

\end{enumerate}


$$T(x,t) = \sum_{n=1}^{\infty} F_n(x) G_n(t) = \sum_{n=1}^{\infty} C_n \cos(n\pi x) e^{- n^2 \pi^2 \alpha^2 t}$$

$\because T(0,x) = f(x)\  \ \therefore \sum_{n=1}^{\infty} C_n \cos(n\pi x) = f(x)$

Now if we multiply both sides this equation by $\cos (m\pi x)$ and integrate:

$\sum_{n=1}^{\infty} C_n \int_0^1 \cos(n\pi x) \cos (m\pi x)= \int_0^1 f(x) \cos (m\pi x)$

$\because \int_0^1 \cos(n\pi x) \cos(m\pi x) dx = \frac{\delta}{2}$
$\therefore C_n \cdot \frac{1}{2} = \int_0^1 f(x) \cos(n\pi x) dx$

we get the final solution:
\begin{equation}
\begin{cases}
T(x,t) =\sum_{n=1}^{\infty} C_n \cos(n\pi x) e^{- n^2 \pi^2 \alpha^2 t}\\[1mm]
C_n = 2\int_0^1 f(x) \cos(n\pi x) dx
\end{cases}
\end{equation}



\bibliographystyle{unsrt}
 
\begin{thebibliography}{99}

\bibitem{KH} 
Kenneth Hardy, 
Linear Algebra for Engineers and Scientists

\bibitem{GJ}
Glyn James, 
Advanced Modern Engineering Mathematics

\end{thebibliography}


\end{document}